\begin{prooftree}
	\Hypo{\Gamma \vdash c1}
	\Hypo {\Gamma \vdash c2}
	\Infer2[and]{\Gamma \vdash c1\ \&\&\ c2}
\end{prooftree}
\quad
\begin{prooftree}
\Hypo{\Gamma \vdash c1}
\Infer1[or(1)]{\Gamma \vdash c1\ ||\ c2}
\end{prooftree}
\quad
\begin{prooftree}
\Hypo{\Gamma \vdash c2}
\Infer1[or(2)]{\Gamma \vdash c1\ ||\ c2}
\end{prooftree}
\quad
\begin{prooftree}
\Hypo{\Gamma \vdash e : \ty{0}{1}}
\Infer1[not]{\Gamma \vdash \neg e : \ty{1}{1}}
\end{prooftree}
\vskip 1cm
\noindent
\begin{prooftree}
\Hypo{\Gamma \vdash e_1 : \nty{t_1}{l_1-h_1}{L_1-H_1}}
\infer[no rule]1{\Gamma \vdash e_2 : \nty{t_2}{l_2-h_2}{L_2-H_2}}
\infer[no rule]1{H_1 <= 4}
\infer[no rule]1{H_2 <= 4}
\infer[no rule]1{h_1 < h_2}
\infer[no rule]1{l_2 > l_1}
%\infer[no rule]1{(t_1 \to t_2) \in \Gamma}
%\infer[no rule]1{Acyclic(\Gamma)}
\Infer1[($<$)]{\Gamma \vdash e_1 < e_2 : \ty{1}{1}}
\end{prooftree}
\quad
\begin{prooftree}
	\Hypo{\Gamma \vdash e : \ty{l-h}{L-H}}
	\infer[no rule]1{l <= l'}
	\infer[no rule]1{h >= h'}
	\infer[no rule]1{L <= L'}
	\infer[no rule]1{H >= H'}
	\infer[no rule]1{l' <= h'}
	\infer[no rule]1{L' <= H'}
	\Infer1[Restriction]{\Gamma \vdash e : \ty{l'-h'}{L'-H'}}
\end{prooftree}
\quad
\begin{prooftree}
	\Hypo{(V_i \mapsto t) \in \Gamma}
	\Infer1[Var store]{\Gamma \vdash V_i : t}
\end{prooftree}